meta_subst_misc.v
@@ -1,0 +1,62 @@
+Require Import util.
+Require Import worlds.
+Require Import meta_term.
+Require Import meta_subst.
+Require Import meta_subst_type.
+Require Import meta_subst_typing.
+Require Import meta_subst_meta_subst.
+Require Import type_assign.
+Require Import meta_subst_type_assign.
+Require Import comp_expr.
+Require Import Coq.Logic.FunctionalExtensionality.
+
+Notation "[[ C1 // X1 ]]" := (msubst_single_t X1 C1) (at level 90). 
+
+Lemma subst_combine : forall {γ δ δ'} (θ:msubst δ γ) (X:δ ↪ δ') C T,
+  ⟦ θ ,, (X, ⟦θ⟧ C) ⟧ T = ⟦θ⟧ ([[ C // X ]] T).
+Admitted.
+
+Theorem subst_lemma : forall {δ δ':world} C U θ (Δ:mtype_assign δ) (Δ':mtype_assign δ'),
+   Δ' ⊩ θ ∷ Δ
+-> Δ  ⊨ C ∷ U
+-> Δ' ⊨ ⟦θ⟧ C ∷ ⟦θ⟧ U.
+Admitted.
+
+Theorem cons_wkn_inv {δ δ' δ'' γ } (θ:msubst δ δ') (X:δ ↪ δ'') (Γ:tp_assign γ δ) C :
+ ⟦θ⟧Γ = ⟦θ ,, (X,C)⟧(import_tp_assign X Γ).
+unfold import_tp_assign.
+erewrite assoc.
+(* TODO: I think there's a nice lemma here... *)
+f_equal.
+unfold compose.
+extensionality y.
+erewrite app_msubst_mvar_result.
+erewrite export_import_inv.
+simpl.
+reflexivity.
+Qed.
+
+
+  Theorem msubst_ext : forall {δ δ' δ'0 α β} (θ : msubst δ β)
+   (X : δ ↪ δ') (θ' : msubst δ β)
+    m  
+   (X0 : δ ↪ δ'0) (T:tp δ'0) (T1:tp δ')  (X' : β ↪ α),
+    ⟦import_msubst X' θ' ,, (X,m_var  X') ⟧ T1 =
+    ⟦import_msubst X' θ ,, (X0, m_var X') ⟧ T ->
+    ⟦θ' ,, (X,m) ⟧ T1 = ⟦θ ,, (X0,m)  ⟧ T.
+   Admitted.
+
+Lemma subst_id {δ} (θ:msubst δ empty) : ⟦·⟧ θ = θ.
+unfold app_subst.
+unfold msubst_substitutable.
+unfold app_subst.
+unfold meta_term_substitutable.
+erewrite app_msubst_id.
+erewrite compose_id_left. reflexivity.
+eexact θ.
+Qed.
+Lemma subst_assoc3 {δ} (T:tp δ) : forall {δ' δ''}
+ (θ:msubst δ δ') (θ':msubst δ' δ''),
+ ⟦⟦θ'⟧θ⟧ T = ⟦θ'⟧(⟦θ⟧T).
+intros. erewrite assoc. reflexivity.
+Qed.
